\nxLnArcBox[]{\bf\nxSFont{12pt}$x + 4 = 7$}
\begin{empheq}[box=\nxWarningMathBox]{align*}
	x + 4 = 7 \\
	x + 4 - 4 = 7 - 4 \\
	x + 0 = 3 \\
\end{empheq}
\bigskip

\nxLnArcBox[]{\bf\nxSFont{12pt}$x + 9 = 15$}
\begin{empheq}[box=\nxWarningMathBox]{align*}
	x + 9 = 15 \\
	x + 9 - 9 = 15 - 9 \\
	x + 0 = 6 \\
\end{empheq}
\bigskip

\nxLnArcBox[]{\bf\nxSFont{12pt}$x + 9 = 15$}
\begin{empheq}[box=\nxWarningMathBox]{align*}
	6 + x = 13 \\
	6 + x - 6 = 15 - 9 \\
	0 + x - 0 = 7 \\
\end{empheq}
\bigskip

\nxLnArcBox[]{\bf\nxSFont{12pt}$x - 3 = 9$}
\begin{empheq}[box=\nxWarningMathBox]{align*}
	x - 3 = 9 \\
	x - 3 + 3 = 9 - 3 \\
	x - 0 = 6 \\
	x = 6 \\
\end{empheq}
\bigskip

\nxLnArcBox[]{\bf\nxSFont{12pt}$x + 8 = 7$}
\begin{empheq}[box=\nxWarningMathBox]{align*}
	x - 8 = 7 \\
	x + 8 - 8 = 7 + 8 \\
	x - 0 = 15 \\
	x = 15 \\
\end{empheq}
\bigskip

\nxLnArcBox[]{\bf\nxSFont{12pt}$6.3 = -2 + x$}
\begin{empheq}[box=\nxWarningMathBox]{align*}
	6.3 = -2 + x \\
	6.3 + 2 = -2 + 2 + x \\
	6.3 = 0 + x \\
	x = 6.3 \\
\end{empheq}
\bigskip

\nxLnArcBox[]{\bf\nxSFont{12pt}$5 = x - 8$}
\begin{empheq}[box=\nxWarningMathBox]{align*}
	5 = x - 8 \\
	5 + 8 = x - 8 + 8 \\
	13 = x - 0 \\
	x = 13 \\
\end{empheq}
\bigskip

\nxLnArcBox[]{\bf\nxSFont{12pt}$5 - x = 12$}
\begin{empheq}[box=\nxWarningMathBox]{align*}
	5 - x = 12\\
	5 - 12 - x + x = 12 - 12 + x\\
	-7 = 0 + x\\
	x = -7\\
\end{empheq}
\bigskip

\nxLnArcBox[]{\bf\nxSFont{12pt}$-8 = 5 - x$}
\begin{empheq}[box=\nxWarningMathBox]{align*}
	-8 = 5 - x\\
	-8 + 8 = 5 + 8 - x\\
	0 + x = 13 - x + x\\
	x = 13
\end{empheq}
\bigskip

\nxLnArcBox[]{\bf\nxSFont{12pt}$3x = 12$}
\begin{empheq}[box=\nxWarningMathBox]{align*}
	3x = 12 \\
	\frac{3x}{3} = \frac{12}{3} \\
	\frac{}{1} = 4 \\
	x = 4 \\
\end{empheq}
\bigskip

\nxLnArcBox[]{\bf\nxSFont{12pt}$7x = 14$}
\begin{empheq}[box=\nxWarningMathBox]{align*}
	7x = 14\\
	\frac{7x}{7} = \frac{12}{7} \\
	\frac{x}{1} = 2 \\
	x = 2 \\
\end{empheq}
\bigskip

\nxLnArcBox[]{\bf\nxSFont{12pt}$-6x = -30$}
\begin{empheq}[box=\nxWarningMathBox]{align*}
	-6x = -30\\
	\frac{-6x}{-6} = \frac{-30}{-6} \\
	\frac{-x}{-1} = 5 \\
	x = 5 \\
\end{empheq}
\bigskip

\nxLnArcBox[]{\bf\nxSFont{12pt}$-6x = -30$}
\begin{empheq}[box=\nxWarningMathBox]{align*}
	-8x = 48\\
	\frac{-8x}{-8} = \frac{48}{-8} \\
	\frac{-x}{-1} = -6 \\
	x = -6 \\
\end{empheq}
\bigskip

\nxLnArcBox[]{\bf\nxSFont{12pt}$7x = -56$}
\begin{empheq}[box=\nxWarningMathBox]{align*}
	7x = -56\\
	\frac{7x}{7} = \frac{-56}{7}\\
	\frac{x}{1} = -8\\
	x = -8\\
\end{empheq}
\bigskip

\nxLnArcBox[]{\bf\nxSFont{12pt}$-8x = -72$}
\begin{empheq}[box=\nxWarningMathBox]{align*}
	-8x = -72 \\
	\frac{-8x}{-8} = \frac{-72}{-8}\\
	\frac{x}{1} = 9 \\
	x = 9 \\
\end{empheq}
\bigskip

