\nxSections{Linear Equations}{3}

\begin{empheq}[box=\nxWarningMathBox]{align*}
	x + 4 = 7 \;\nxArw{5}\;
	x + 4 - 4 = 7 - 4  \;\nxArw{5}\;
	x + 0 = 3
\end{empheq}
\begin{empheq}[box=\nxWarningMathBox]{align*}
	x + 9 = 15 \;\nxArw{5}\;
	x + 9 - 9 = 15 - 9 \;\nxArw{5}\;
	x + 0 = 6
\end{empheq}
\begin{empheq}[box=\nxWarningMathBox]{align*}
	6 + x = 13 \;\nxArw{5}\;
	6 + x - 6 = 15 - 9 \;\nxArw{5}\;
	0 + x - 0 = 7
\end{empheq}
\begin{empheq}[box=\nxWarningMathBox]{align*}
	x - 3 = 9 \;\nxArw{5}\;
	x - 3 + 3 = 9 - 3  \;\nxArw{5}\;
	x - 0 = 6 \;\nxArw{5}\;
	x = 6
\end{empheq}
\begin{empheq}[box=\nxWarningMathBox]{align*}
	x - 8 = 7  \;\nxArw{5}\;
	x + 8 - 8 = 7 + 8  \;\nxArw{5}\;
	x - 0 = 15 \;\nxArw{5}\;
	x = 15
\end{empheq}
\begin{empheq}[box=\nxWarningMathBox]{align*}
	6.3 = -2 + x  \;\nxArw{5}\;
	6.3 + 2 = -2 + 2 + x \;\nxArw{5}\;
	6.3 = 0 + x \;\nxArw{5}\;
	x = 6.3
\end{empheq}
\begin{empheq}[box=\nxWarningMathBox]{align*}
	5 = x - 8 \;\nxArw{5}\;
	5 + 8 = x - 8 + 8  \;\nxArw{5}\;
	13 = x - 0  \;\nxArw{5}\;
	x = 13
\end{empheq}
\begin{empheq}[box=\nxWarningMathBox]{align*}
	5 - x = 12 \;\nxArw{5}\;
	5 - 12 - x + x = 12 - 12 + x \;\nxArw{5}\;\\\nxArw{22}
	-7 = 0 + x \;\nxArw{5}\;
	x = -7
\end{empheq}
\begin{empheq}[box=\nxWarningMathBox]{align*}
	-8 = 5 - x \;\nxArw{5}\;
	-8 + 8 = 5 + 8 - x \;\nxArw{5}\;\\\nxArw{22}
	0 + x = 13 - x + x \;\nxArw{5}\;
	x = 13
\end{empheq}
\begin{empheq}[box=\nxWarningMathBox]{align*}
	3x = 12 \;\nxArw{5}\;
	\frac{3x}{3} = \frac{12}{3} \;\nxArw{5}\;
	\frac{}{1} = 4 \;\nxArw{5}\;
	x = 4
\end{empheq}
\begin{empheq}[box=\nxWarningMathBox]{align*}
	7x = 14 \;\nxArw{5}\;
	\frac{7x}{7} = \frac{12}{7} \;\nxArw{5}\;
	\frac{x}{1} = 2 \;\nxArw{5}\;
	x = 2
\end{empheq}
\begin{empheq}[box=\nxWarningMathBox]{align*}
	-6x = -30 \;\nxArw{5}\;
	\frac{-6x}{-6} = \frac{-30}{-6} \;\nxArw{5}\;
	\frac{-x}{-1} = 5 \;\nxArw{5}\;
	x = 5
\end{empheq}
\begin{empheq}[box=\nxWarningMathBox]{align*}
	-8x = 48 \;\nxArw{5}\;
	\frac{-8x}{-8} = \frac{48}{-8} \;\nxArw{5}\;
	\frac{-x}{-1} = -6 \;\nxArw{5}\;
	x = -6
\end{empheq}
\begin{empheq}[box=\nxWarningMathBox]{align*}
	7x = -56 \;\nxArw{5}\;
	\frac{7x}{7} = \frac{-56}{7} \;\nxArw{5}\;
	\frac{x}{1} = -8 \;\nxArw{5}\;
	x = -8
\end{empheq}
\begin{empheq}[box=\nxWarningMathBox]{align*}
	-8x = -72 \;\nxArw{5}\;
	\frac{-8x}{-8} = \frac{-72}{-8} \;\nxArw{5}\;
	\frac{x}{1} = 9 \;\nxArw{5}\;
	x = 9
\end{empheq}
\bigskip

